Initializers: Minor improvements
- Add monotonicity wrt `sub_module`
- Prove `Proper` instances
- Factor out `wp_initialize_unqualified`
- Add `wp_initialize_ok`
- Make definitions opaque in `typeclass_instances`
- Prefer `cQp.mk (q_const cv) 1` to a match on `q_const cv`

theories/lang/cpp/logic/initializers.v
@@ -33,7 +33,152 @@ Note that the frontend inserts constructor calls to default initialize
 objects, so [Tnamed] types can *not* be default initialized.
 *)
 
-Section with_resolve.
+(** ** Default initilalization *)
+(**
+[default_initialize_array default_initialize tu ty len p Q]
+initializes an array of type [ty[len]] at pointer [p] using
+[default_initialize].
+
+NOTE that default initialization of an array of constants is a
+compile-time error, so we don't need to worry about that case.
+Also, note that arrays of length 0 are not legal so we are
+guaranteed to have to initialize a value which will result in an
+[ERROR].
+*)
+Definition default_initialize_array `{Σ : cpp_logic, σ : genv}
+    (default_initialize : translation_unit -> type -> ptr -> (FreeTemps -> epred) -> mpred)
+    (tu : translation_unit) (ty : type) (len : N) (p : ptr) (Q : FreeTemps -> epred) : mpred :=
+  let folder i PP :=
+    default_initialize tu ty (p ,, o_sub _ ty (Z.of_N i)) (fun free' => interp tu free' PP)
+  in
+  foldr folder (p .[ ty ! Z.of_N len ] |-> validR -* Q FreeTemps.id) (seqN 0 len).
+#[global] Hint Opaque default_initialize_array : typeclass_instances.
+#[global] Arguments default_initialize_array : simpl never.
+
+(**
+[default_initialize tu ty p Q] default initializes the memory at [p]
+according to the type [ty].
+
+NOTE this assumes that the underlying memory has already been given to
+the C++ abstract machine.
+
+NOTE: <https://eel.is/c++draft/dcl.init#general-7>:
+| (7) To default-initialize an object of type T means:
+| (7.1) If T is a (possibly cv-qualified) class type ([class]), constructors are considered.
+|       The applicable constructors are enumerated ([over.match.ctor]), and the best one for
+|       the initializer () is chosen through overload resolution ([over.match]).
+|       The constructor thus selected is called, with an empty argument list, to initialize
+|       the object.
+| (7.2) If T is an array type, each element is default-initialized.
+| (7.3) Otherwise, no initialization is performed.
+
+and [default_initialize] corresponds to [default-initialization] as
+described above.
+*)
+Fixpoint default_initialize `{Σ : cpp_logic, σ : genv} (tu : translation_unit)
+    (ty : type) (p : ptr) (Q : FreeTemps → epred) {struct ty} : mpred :=
+  match ty with
+  | Tnum _ _
+  | Tchar_ _
+  | Tptr _
+  | Tbool
+  | Tfloat_ _
+  | Tnullptr
+  | Tenum _ =>
+    let rty := erase_qualifiers ty in
+    p |-> uninitR rty (cQp.m 1) -* Q FreeTemps.id
+
+  | Tarray ety sz =>
+    default_initialize_array default_initialize tu ety sz p (fun _ => Q FreeTemps.id)
+
+  | Tref _
+  | Trv_ref _ => ERROR "default initialization of reference"
+  | Tvoid => ERROR "default initialization of void"
+  | Tfunction _ _ => ERROR "default initialization of functions"
+  | Tmember_pointer _ _ => ERROR "default initialization of member pointers"
+  | Tnamed _ => False (* default initialization of aggregates is done at elaboration time. *)
+
+  | Tarch _ _ => UNSUPPORTED "default initialization of architecture type"
+  | Tqualified q ty =>
+    if q_const q then ERROR "default initialize const"
+    else default_initialize tu ty p Q
+  end%bs%I.
+#[global] Hint Opaque default_initialize : typeclass_instances.
+#[global] Arguments default_initialize _ _ _ _ !_ _ _ / : assert.
+
+Section frame.
+  Context `{Σ : cpp_logic, σ : genv}.
+  Implicit Types (Q : FreeTemps -> epred).
+  Implicit Types (di : translation_unit -> type -> ptr -> (FreeTemps -> epred) -> mpred).
+
+  Lemma default_initialize_array_frame di tu tu' ty sz Q Q' (p : ptr) :
+    sub_module tu tu' ->
+    (∀ p Q Q', (Forall f, Q f -* Q' f) |-- di tu ty p Q -* di tu' ty p Q') ->
+    (Forall f, Q f -* Q' f)
+    |-- default_initialize_array di tu ty sz p Q -* default_initialize_array di tu' ty sz p Q'.
+  Proof.
+    intros Hsub IHty.
+    rewrite /default_initialize_array.
+    generalize dependent (p .[ ty ! Z.of_N sz ] |-> validR).
+    induction (seqN 0 sz) =>/=; intros.
+    - iIntros "X a b". iApply "X". by iApply "a".
+    - iIntros "F". iApply IHty.
+      iIntros (?). iApply interp_frame_strong; [done|]. iApply (IHl with "F").
+  Qed.
+
+  (**
+  TODO this should be generalized to different [σ] but, in that case
+  it relies on the fact that [ty] is defined in both environments.
+  *)
+  Lemma default_initialize_frame tu tu' ty this Q Q' :
+    sub_module tu tu' ->
+    (Forall f, Q f -* Q' f)
+    |-- default_initialize tu ty this Q -* default_initialize tu' ty this Q'.
+  Proof.
+    intros.
+    move: this Q Q'. induction ty=>this Q Q'; simpl; intros; try case_match;
+      try solve [ intros; iIntros "a b c"; iApply "a"; iApply "b"; eauto | eauto ].
+    { intros. iIntros "a". by iApply (default_initialize_array_frame with "a"). }
+  Qed.
+
+  #[global] Instance: Params (@default_initialize) 6 := {}.
+  #[local] Notation INIT R := (
+    ∀ tu ty this,
+    Proper (pointwise_relation _ R ==> R) (default_initialize tu ty this)
+  ) (only parsing).
+  #[global] Instance default_initialize_mono : INIT bi_entails.
+  Proof.
+    intros * Q1 Q2 HQ. iIntros "wp".
+    iApply (default_initialize_frame with "[] wp"); [done|]. iIntros (free) "Q".
+    by iApply HQ.
+  Qed.
+  #[global] Instance default_initialize_flip_mono : INIT (flip bi_entails).
+  Proof. repeat intro. by apply default_initialize_mono. Qed.
+  #[global] Instance default_initialize_proper : INIT equiv.
+  Proof. intros * Q1 Q2 HQ. by split'; apply default_initialize_mono=>free; rewrite HQ. Qed.
+
+  #[global] Instance: Params (@default_initialize_array) 8 := {}.
+  #[local] Notation ARRAY R := (
+    ∀ tu ty sz p,
+    Proper (pointwise_relation _ R ==> R)
+      (default_initialize_array default_initialize tu ty sz p)
+  ) (only parsing).
+  #[global] Instance default_initialize_array_mono : ARRAY bi_entails.
+  Proof.
+    intros * Q1 Q2 HQ. iIntros "wp".
+    iApply (default_initialize_array_frame with "[] wp"); [done| |].
+    { clear=>p Q Q'. exact: default_initialize_frame. }
+    { iIntros (free) "Q". by iApply HQ. }
+  Qed.
+  #[global] Instance default_initialize_array_flip_mono : ARRAY (flip bi_entails).
+  Proof. repeat intro. by apply default_initialize_array_mono. Qed.
+  #[global] Instance default_initialize_array_proper : ARRAY equiv.
+  Proof. intros * Q1 Q2 HQ. by split'; apply default_initialize_array_mono=>free; rewrite HQ. Qed.
+End frame.
+
+(** ** Expression initialization *)
+
+Section wp_initialize.
   Context `{Σ : cpp_logic thread_info} {σ:genv} (tu : translation_unit).
   Implicit Types (Q : FreeTemps -> epred).
   Variables (ρ : region).
@@ -46,101 +191,6 @@ Section with_resolve.
   #[local] Notation interp := (interp tu).
   #[local] Notation wp_fptr := (@wp_fptr _ Σ tu.(types)).
   #[local] Notation mspec := (@mspec _ Σ tu.(types)).
-
-  (**
-  [default_initialize_array default_init ty len p Q] initializes an
-  array of type [ty[len]] at pointer [p].
-
-  NOTE that default initialization of an array of constants is a
-  compile-time error, so we don't need to worry about that case.
-  Also, note that arrays of length 0 are not legal so we are
-  guaranteed to have to initialize a value which will result in an
-  [ERROR].
-  *)
-  Definition default_initialize_array
-      (default_initialize : type -> ptr -> (FreeTemps -> epred) -> mpred)
-      (ty : type) (len : N) (p : ptr) (Q : FreeTemps -> epred) : mpred :=
-    let folder i PP :=
-      default_initialize ty (p ,, o_sub _ ty (Z.of_N i)) (fun free' => interp free' PP)
-    in
-    foldr folder (p .[ ty ! Z.of_N len ] |-> validR -* Q FreeTemps.id) (seqN 0 len).
-  #[global] Arguments default_initialize_array : simpl never.
-
-  Lemma default_initialize_array_frame di ty sz Q Q' (p : ptr) :
-    (∀ p Q Q', (Forall f, Q f -* Q' f) |-- di ty p Q -* di ty p Q') ->
-    (Forall f, Q f -* Q' f)
-    |-- default_initialize_array di ty sz p Q -* default_initialize_array di ty sz p Q'.
-  Proof.
-    intros IHty.
-    rewrite /default_initialize_array.
-    generalize dependent (p .[ ty ! Z.of_N sz ] |-> validR).
-    induction (seqN 0 sz) =>/=; intros.
-    - iIntros "X a b". iApply "X". by iApply "a".
-    - iIntros "F". iApply IHty.
-      iIntros (?). iApply interp_frame. iApply (IHl with "F").
-  Qed.
-
-  (**
-  [default_initialize ty p Q] default initializes the memory at [p]
-  according to the type [ty].
-
-  NOTE this assumes that the underlying memory has already been
-  given to the C++ abstract machine.
-
-  NOTE: <https://eel.is/c++draft/dcl.init#general-7>:
-  | (7) To default-initialize an object of type T means:
-  | (7.1) If T is a (possibly cv-qualified) class type ([class]), constructors are considered.
-  |       The applicable constructors are enumerated ([over.match.ctor]), and the best one for
-  |       the initializer () is chosen through overload resolution ([over.match]).
-  |       The constructor thus selected is called, with an empty argument list, to initialize
-  |       the object.
-  | (7.2) If T is an array type, each element is default-initialized.
-  | (7.3) Otherwise, no initialization is performed.
-
-  and [default_initialize] corresponds to [default-initialization]
-  as described above.
-  *)
-  Fixpoint default_initialize (ty : type) (p : ptr) (Q : FreeTemps → epred) {struct ty} : mpred :=
-    match ty with
-    | Tnum _ _
-    | Tchar_ _
-    | Tptr _
-    | Tbool
-    | Tfloat_ _
-    | Tnullptr
-    | Tenum _ =>
-      let rty := erase_qualifiers ty in
-      p |-> uninitR rty (cQp.m 1) -* Q FreeTemps.id
-
-    | Tarray ety sz =>
-      default_initialize_array default_initialize ety sz p (fun _ => Q FreeTemps.id)
-
-    | Tref _
-    | Trv_ref _ => ERROR "default initialization of reference"
-    | Tvoid => ERROR "default initialization of void"
-    | Tfunction _ _ => ERROR "default initialization of functions"
-    | Tmember_pointer _ _ => ERROR "default initialization of member pointers"
-    | Tnamed _ => False (* default initialization of aggregates is done at elaboration time. *)
-
-    | Tarch _ _ => UNSUPPORTED "default initialization of architecture type"
-    | Tqualified q ty =>
-      if q_const q then ERROR "default initialize const"
-      else default_initialize ty p Q
-    end%bs%I.
-  #[global] Arguments default_initialize !_ _ _ / : assert.
-
-  (**
-  TODO this should be generalized to different [σ] but, in that case
-  it relies on the fact that [ty] is defined in both environments.
-  *)
-  Lemma default_initialize_frame ty : forall this Q Q',
-    (Forall f, Q f -* Q' f)
-    |-- default_initialize ty this Q -* default_initialize ty this Q'.
-  Proof.
-    induction ty; simpl; intros; try case_match;
-      try solve [ intros; iIntros "a b c"; iApply "a"; iApply "b"; eauto | eauto ].
-    { intros. iIntros "a". by iApply (default_initialize_array_frame with "a"). }
-  Qed.
 
   (* error used when using [e] to initialize a value of type [ty]. *)
   Variant initializing_type (ty : type) (e : Expr) : Prop := ANY.
@@ -159,14 +209,15 @@ Section with_resolve.
   references) whereas [wp_init] is only safe to initialize
   non-primitives (arrays and aggregates).
   *)
-  Definition wp_initialize (qty : type) (addr : ptr) (init : Expr) (Q : FreeTemps -> mpred) : mpred :=
-    let '(cv, ty) := decompose_type qty in
-    (**
-    TODO (Gregory): In a few cases below, we're using [cQp.m 1]
-    rather than [qf]. Please add a comment explaining.
-    *)
-    let qf := if q_const cv then cQp.const 1 else cQp.mut 1 in
+  Definition wp_initialize_unqualified (cv : type_qualifiers) (ty : type)
+      (addr : ptr) (init : Expr) (Q : FreeTemps -> epred) : mpred :=
     match ty with
+
+    (**
+    Note: For primitive types, we effectively bake in [if q_const cv
+    then wp_make_const tu addr ty else id].
+    *)
+
     | Tvoid =>
       (*
       [wp_initialize] is used to `return` from a function. The
@@ -177,6 +228,7 @@ Section with_resolve.
       >>
       *)
       letI* v, frees := wp_operand init in
+      let qf := cQp.mk (q_const cv) 1 in
       [| v = Vvoid |] **
       (addr |-> primR Tvoid qf Vvoid -* Q frees)
 
@@ -189,6 +241,7 @@ Section with_resolve.
     | Tfloat_ _
     | Tnullptr =>
       letI* v, free := wp_operand init in
+      let qf := cQp.mk (q_const cv) 1 in
       addr |-> primR (erase_qualifiers ty) qf v -* Q free
 
       (* non-primitives are handled via prvalue-initialization semantics *)
@@ -201,6 +254,7 @@ Section with_resolve.
     | Tref ty =>
       let rty := Tref $ erase_qualifiers ty in
       letI* p, free := wp_lval init in
+      let qf := cQp.mk (q_const cv) 1 in
       (*
       TODO: [ref]s are never mutable, but we use [qf] here
       for compatibility with [implicit_destruct_struct]
@@ -210,6 +264,7 @@ Section with_resolve.
     | Trv_ref ty =>
       let rty := Tref $ erase_qualifiers ty in
       letI* p, free := wp_xval init in
+      let qf := cQp.mk (q_const cv) 1 in
       (*
       TODO: [ref]s are never mutable, but we use [qf] here
       for compatibility with [implicit_destruct_struct]
@@ -221,7 +276,29 @@ Section with_resolve.
     | Tqualified _ ty => False (* unreachable *)
     | Tarch _ _ => UNSUPPORTED (initializing_type ty init)
     end.
-  #[global] Arguments wp_initialize !_ _ _ _ /.
+  #[global] Hint Opaque wp_initialize_unqualified : typeclass_instances.
+  #[global] Arguments wp_initialize_unqualified _ !_ _ _ _ / : assert.
+
+  Definition wp_initialize (qty : type) (addr : ptr) (init : Expr) (Q : FreeTemps -> epred) : mpred :=
+    qual_norm wp_initialize_unqualified qty addr init Q.
+  #[global] Hint Opaque wp_initialize : typeclass_instances.
+  #[global] Arguments wp_initialize !_ _ _ _ / : assert.
+
+  Lemma wp_initialize_ok qty :
+    qual_norm_spec wp_initialize_unqualified QM qty (wp_initialize qty).
+  Proof. apply qual_norm_ok. Qed.
+
+  Lemma wp_initialize_qual_norm qty :
+    wp_initialize qty = qual_norm wp_initialize_unqualified qty.
+  Proof. done. Qed.
+
+  Lemma wp_initialize_decompose_type qty :
+    wp_initialize qty =
+      let p := decompose_type qty in
+      wp_initialize_unqualified p.1 p.2.
+  Proof.
+    by rewrite wp_initialize_qual_norm qual_norm_decompose_type.
+  Qed.
 
   (**
   [wpi cls this init Q] evaluates the initializer [init] from the
@@ -239,61 +316,120 @@ Section with_resolve.
     letI* free := wp_initialize init.(init_type) p' init.(init_init) in
     letI* := interp free in
     Q.
-  #[global] Arguments wpi _ _ _ _ /.
+  #[global] Hint Opaque wpi : typeclass_instances.
+  #[global] Arguments wpi _ _ _ _ / : assert.
 
-End with_resolve.
+End wp_initialize.
 
-#[global] Hint Opaque default_initialize_array : typeclass_instances.
+(*
+All framing lemmas *should* work with [genv] weakening, but that
+requires some additional side-conditions on paths that we can't prove
+right now. So, for the time being, we prove [_frame] lemmas without
+[genv] weakening.
+*)
 
 Section frames.
-  Context `{Σ : cpp_logic thread_info} {σ1 σ2 :genv} (tu : translation_unit).
-  Variables (ρ : region).
-  Hypothesis MOD : genv_leq σ1 σ2.
+  Context `{Σ : cpp_logic thread_info, σ : genv}.
+  Implicit Types (Q : FreeTemps -> epred).
 
-  Lemma wp_initialize_frame obj ty e Q Q' :
+  Lemma wp_initialize_unqualified_frame tu tu' ρ obj cv ty e Q Q' :
+    sub_module tu tu' ->
     (Forall free, Q free -* Q' free)
-    |-- wp_initialize (σ:=σ2) tu ρ ty obj e Q -* wp_initialize (σ:=σ2) tu ρ ty obj e Q'.
-  Proof using.
-    rewrite /wp_initialize.
-    iIntros "a".
-    case: (decompose_type _)=>a; case=>>; auto; try
-        by [ iApply wp_operand_frame => //; iIntros (??) "X ?"; iApply "a"; iApply "X"
-           | iIntros "H"; iExact "H"
-           | iApply wp_init_frame => //-;
-             case: (q_const _); iIntros (??); [ iApply wp_const_frame; try reflexivity | ]; iApply "a"
-           ].
-    { by iApply wp_lval_frame => //; iIntros (??) "X ?"; iApply "a"; iApply "X". }
-    { by iApply wp_xval_frame => //; iIntros (??) "X ?"; iApply "a"; iApply "X". }
-    { by iApply wp_operand_frame => //; iIntros (??) "[$ X] ?"; iApply "a"; iApply "X". }
+    |-- wp_initialize_unqualified tu ρ cv ty obj e Q -* wp_initialize_unqualified tu' ρ cv ty obj e Q'.
+  Proof.
+    intros. iIntros "HQ'". destruct ty; cbn; auto.
+    all:
+      lazymatch goal with
+      | |- context [wp_operand] => iApply wp_operand_frame; [done|]
+      | |- context [wp_lval] => iApply wp_lval_frame; [done|]
+      | |- context [wp_xval] => iApply wp_xval_frame; [done|]
+      | |- context [wp_init] => iApply wp_init_frame; [done|]
+      | _ => idtac
+      end;
+      try by iIntros (??) "HQ ?"; iApply "HQ'"; iApply "HQ".
+    all:
+      lazymatch goal with
+      | |- context [wp_const] =>
+        iIntros (??);
+        destruct (q_const cv);
+          [ iApply wp_const_frame; [exact: types_compat|]
+          | cbn ];
+        iIntros "?"; by iApply "HQ'"
+      | _ => idtac
+      end.
+    (* void *)
+    iIntros (??) "($ & HQ) ?". iApply "HQ'". by iApply "HQ".
   Qed.
 
-  Lemma wp_initialize_wand obj ty e Q Q' :
-    wp_initialize (σ:=σ2) tu ρ ty obj e Q
-    |-- (Forall free, Q free -* Q' free) -* wp_initialize (σ:=σ2) tu ρ ty obj e Q'.
+  #[global] Instance: Params (@wp_initialize_unqualified) 9 := {}.
+  #[local] Notation BODY R := (
+    ∀ tu ρ cv ty obj init,
+    Proper (pointwise_relation _ R ==> R) (wp_initialize_unqualified tu ρ cv ty obj init)
+  ) (only parsing).
+  #[global] Instance wp_initialize_unqualified_mono : BODY bi_entails.
+  Proof.
+    intros * Q1 Q2 HQ. iIntros "wp".
+    iApply (wp_initialize_unqualified_frame with "[] wp"); [done|]. iIntros (free) "Q".
+    by iApply HQ.
+  Qed.
+  #[global] Instance wp_initialize_unqualified_flip_mono : BODY (flip bi_entails).
+  Proof. repeat intro. by apply wp_initialize_unqualified_mono. Qed.
+  #[global] Instance wp_initialize_unqualified_proper : BODY equiv.
+  Proof. intros * Q1 Q2 HQ. by split'; apply wp_initialize_unqualified_mono=>free; rewrite HQ. Qed.
+
+  Lemma wp_initialize_frame tu tu' ρ obj ty e Q Q' :
+    sub_module tu tu' ->
+    (Forall free, Q free -* Q' free)
+    |-- wp_initialize tu ρ ty obj e Q -* wp_initialize tu' ρ ty obj e Q'.
+  Proof using.
+    intros. rewrite /wp_initialize/qual_norm.
+    induction (wp_initialize_ok tu ρ ty); last done.
+    rewrite !qual_norm'_unqual. exact: wp_initialize_unqualified_frame.
+  Qed.
+
+  #[global] Instance: Params (@wp_initialize) 8 := {}.
+  #[local] Notation INIT R := (
+    ∀ tu ρ ty obj init,
+    Proper (pointwise_relation _ R ==> R) (wp_initialize tu ρ ty obj init)
+  ) (only parsing).
+  #[global] Instance wp_initialize_mono : INIT bi_entails.
+  Proof.
+    intros * Q1 Q2 HQ. iIntros "wp".
+    iApply (wp_initialize_frame with "[] wp"); [done|]. iIntros (free) "Q".
+    by iApply HQ.
+  Qed.
+  #[global] Instance wp_initialize_flip_mono : INIT (flip bi_entails).
+  Proof. repeat intro. by apply wp_initialize_mono. Qed.
+  #[global] Instance wp_initialize_proper : INIT equiv.
+  Proof. intros * Q1 Q2 HQ. by split'; apply wp_initialize_mono=>free; rewrite HQ. Qed.
+
+  Lemma wp_initialize_wand tu ρ obj ty e Q Q' :
+    wp_initialize tu ρ ty obj e Q
+    |-- (Forall free, Q free -* Q' free) -* wp_initialize tu ρ ty obj e Q'.
   Proof. by iIntros "H Y"; iRevert "H"; iApply wp_initialize_frame. Qed.
 
-  Theorem wpi_frame (cls : globname) (this : ptr) (e : Initializer) k1 k2 :
-    k1 -* k2 |-- wpi (σ:=σ1) tu ρ cls this e k1 -* wpi (σ:=σ2) tu ρ cls this e k2.
-  Proof. Abort. (* This is not provable *)
-End frames.
-
-Section mono_frames.
-  (*
-  All framing lemmas *should* work with [genv] weakening, but that
-  requires some additional side-conditions on paths that we can't
-  prove right now. So, for the time being, we prove [_frame] lemmas
-  without [genv] weakening.
-  *)
-
-  Context `{Σ : cpp_logic thread_info} {σ : genv} (tu : translation_unit).
-  Variables (ρ : region).
-
-  Theorem wpi_frame (cls : globname) (this : ptr) (e : Initializer) k1 k2 :
-    k1 -* k2 |-- wpi tu ρ cls this e k1 -* wpi tu ρ cls this e k2.
+  Lemma wpi_frame tu tu' ρ cls this e (Q Q' : epred) :
+    sub_module tu tu' ->
+    Q -* Q' |-- wpi tu ρ cls this e Q -* wpi tu' ρ cls this e Q'.
   Proof.
-    clear.
-    iIntros "X". rewrite /wpi. iApply wp_initialize_frame.
-    iIntros (?); by iApply interp_frame.
+    intros. iIntros "HQ". rewrite /wpi.
+    iApply wp_initialize_frame; [done|]. iIntros (free).
+    by iApply interp_frame_strong.
   Qed.
 
-End mono_frames.
+  #[global] Instance: Params (@wpi) 8 := {}.
+  #[local] Notation WPI R := (
+    ∀ tu ρ cls this e,
+    Proper (R ==> R) (wpi tu ρ cls this e)
+  ) (only parsing).
+  #[global] Instance wpi_mono : WPI bi_entails.
+  Proof.
+    intros * Q1 Q2 HQ. iIntros "wp".
+    iApply (wpi_frame with "[] wp"); [done|]. iIntros "Q".
+    by iApply HQ.
+  Qed.
+  #[global] Instance wpi_flip_mono : WPI (flip bi_entails).
+  Proof. repeat intro. by apply wpi_mono. Qed.
+  #[global] Instance wpi_proper : WPI equiv.
+  Proof. intros * Q1 Q2 HQ. by split'; apply wpi_mono; rewrite HQ. Qed.
+End frames.
